Given_Clause_Loops/Zipperposition_Loop.thy
@@ -16,7 +16,7 @@ begin
 
 subsection \<open>Definition and Lemmas\<close>
 
-fun flat_inferences_of :: "'f inference llist set \<Rightarrow> 'f inference set " where
+fun flat_inferences_of :: "'f inference llist set \<Rightarrow> 'f inference set" where
   "flat_inferences_of T = \<Union> {lset x |x. x \<in> T}"
 
 fun
